Still more stack work (finished progress)

02Stack/Stack.thy
@@ -1,32 +1,50 @@
 theory Stack
-imports "../Vector" "../01Expression/Expression"
+imports "../Heap" "../01Expression/Expression"
 begin
+
+datatype val = 
+  VAbs type expr
+| VRec "nat list"
+| VInj nat "type list" nat
+| VFold type nat
+| VTyAbs kind expr
 
 datatype frame = 
   SRef nat
 | SApp expr
-| SBind
 | SProj nat
 | SCase type "expr list"
 | SUnfold type
 | STyApp type
 
-datatype stack_direction = Eval | Return
+datatype focus = 
+  Eval expr 
+| Return val
 
-datatype stack_state = StackState stack_direction expr "frame list" "expr list"
+datatype stack_state = StackState focus "frame list" "expr heap"
 
-fun unstack :: "expr \<Rightarrow> frame list \<Rightarrow> expr list \<Rightarrow> expr" where
+primrec devalue :: "val \<Rightarrow> expr" where
+  "devalue (VAbs t e) = Abs t e"
+| "devalue (VRec xs) = Rec (map Var xs)"
+| "devalue (VInj l ts x) = Inj l ts (Var x)"
+| "devalue (VFold t x) = Fold t (Var x)"
+| "devalue (VTyAbs k e) = TyAbs k e"
+
+fun devar :: "expr \<Rightarrow> nat" where
+  "devar (Var x) = x"
+| "devar _ = undefined"
+
+fun unstack :: "expr \<Rightarrow> frame list \<Rightarrow> expr heap \<Rightarrow> expr" where
   "unstack e [] h = e"
-| "unstack e (SRef x # s) h = unstack (Var x) s (update_at x e h)"
+| "unstack e (SRef x # s) h = unstack (Var x) s (update\<^sub>h h x e)"
 | "unstack e (SApp e' # s) h = unstack (App e e') s h"
-| "unstack e (SBind # s) [] = undefined"
-| "unstack e (SBind # s) (e' # h) = unstack (Let e' e) s h"
 | "unstack e (SProj l # s) h = unstack (Proj e l) s h"
 | "unstack e (SCase t cs # s) h = unstack (Case e t cs) s h"
 | "unstack e (SUnfold t # s) h = unstack (Unfold t e) s h"
 | "unstack e (STyApp t # s) h = unstack (TyApp e t) s h"
 
-primrec unstack_state :: "stack_state \<Rightarrow> expr" where
-  "unstack_state (StackState _ e s h) = unstack e s h"
+fun unstack_state :: "stack_state \<Rightarrow> expr" where
+  "unstack_state (StackState (Eval e) s h) = unstack e s h"
+| "unstack_state (StackState (Return v) s h) = unstack (devalue v) s h"
 
 end
