02Stack/TypecheckStack.thy
@@ -2,86 +2,115 @@ theory TypecheckStack
 imports Stack "../01Expression/Typecheck"
 begin
 
-inductive typecheck_frame :: "type list \<Rightarrow> frame \<Rightarrow> type list \<Rightarrow> type \<Rightarrow> type \<Rightarrow> bool" 
-    (infix "\<turnstile>\<^sub>s _ : _,_ \<rightarrow>" 60) where
-  tc_sref [simp]: "lookup x \<Gamma> = Some t \<Longrightarrow> \<Gamma> \<turnstile>\<^sub>s SRef x : \<Gamma>,t \<rightarrow> t"
-| tc_sapp [simp]: "[],\<Gamma> \<turnstile> e : t' \<Longrightarrow> \<Gamma> \<turnstile>\<^sub>s SApp e : \<Gamma>,Arrow t' t \<rightarrow> t"
-| tc_sbind [simp]: "\<Gamma> \<turnstile>\<^sub>s SBind : t' # \<Gamma>,t \<rightarrow> t"
-| tc_sproj [simp]: "lookup l ts = Some t \<Longrightarrow> \<Gamma> \<turnstile>\<^sub>s SProj l : \<Gamma>,Record ts \<rightarrow> t"
-| tc_scase [simp]: "[],\<Gamma> \<turnstile>\<^sub>c cs : ts \<rightarrow> t \<Longrightarrow> \<Gamma> \<turnstile>\<^sub>s SCase t cs : \<Gamma>,Variant ts \<rightarrow> t"
-| tc_sunfold [simp]: "[k] \<turnstile>\<^sub>k t : Star \<Longrightarrow> 
-    \<Gamma> \<turnstile>\<^sub>s SUnfold t : \<Gamma>,Inductive k t \<rightarrow> subst\<^sub>t\<^sub>t 0 (Inductive k t) t"
-| tc_styapp [simp]: "[] \<turnstile>\<^sub>k t' : k \<Longrightarrow> \<Gamma> \<turnstile>\<^sub>s STyApp t' : \<Gamma>,Forall k t \<rightarrow> subst\<^sub>t\<^sub>t 0 t' t"
+inductive typecheck_value :: "kind list \<Rightarrow> type list \<Rightarrow> val \<Rightarrow> type \<Rightarrow> bool" (infix ",_ \<turnstile>\<^sub>v _ :" 60) 
+      and typecheck_vars :: "kind list \<Rightarrow> type list \<Rightarrow> nat list \<Rightarrow> type list \<Rightarrow> bool" 
+        (infix ",_ \<turnstile>\<^sub>v\<^sub>s _ :" 60) where
+  tc_vabs [simp]: "\<Delta>,insert_at 0 t\<^sub>1 \<Gamma> \<turnstile> e : t\<^sub>2 \<Longrightarrow> \<Delta> \<turnstile>\<^sub>k t\<^sub>1 : Star \<Longrightarrow> \<Delta>,\<Gamma> \<turnstile>\<^sub>v VAbs t\<^sub>1 e : Arrow t\<^sub>1 t\<^sub>2"
+| tc_vrec [simp]: "\<Delta>,\<Gamma> \<turnstile>\<^sub>v\<^sub>s fs : ts \<Longrightarrow> \<Delta>,\<Gamma> \<turnstile>\<^sub>v VRec fs : Record ts"
+| tc_vinj [simp]: "lookup x \<Gamma> = Some t \<Longrightarrow> lookup l ts = Some t \<Longrightarrow> \<forall>tt \<in> set ts. \<Delta> \<turnstile>\<^sub>k tt : Star \<Longrightarrow> 
+    \<Delta>,\<Gamma> \<turnstile>\<^sub>v VInj l ts x : Variant ts"
+| tc_vfold [simp]: "lookup x \<Gamma> = Some (subst\<^sub>t\<^sub>t 0 (Inductive k t) t) \<Longrightarrow> 
+    insert_at 0 k \<Delta> \<turnstile>\<^sub>k t : Star \<Longrightarrow> \<Delta>,\<Gamma> \<turnstile>\<^sub>v VFold t x : Inductive k t"
+| tc_vtyabs [simp]: "insert_at 0 k \<Delta>,map (incr\<^sub>t\<^sub>t 0) \<Gamma> \<turnstile> e : t \<Longrightarrow> \<Delta>,\<Gamma> \<turnstile>\<^sub>v VTyAbs k e : Forall k t"
+| tc_vnil [simp]: "\<Delta>,\<Gamma> \<turnstile>\<^sub>v\<^sub>s [] : []"
+| tc_vcons [simp]: "lookup x \<Gamma> = Some t \<Longrightarrow> \<Delta>,\<Gamma> \<turnstile>\<^sub>v\<^sub>s vs : ts \<Longrightarrow> \<Delta>,\<Gamma> \<turnstile>\<^sub>v\<^sub>s x # vs : t # ts"
 
-inductive_cases [elim]: "\<Gamma> \<turnstile>\<^sub>s SRef x : \<Gamma>',t \<rightarrow> t'"
-inductive_cases [elim]: "\<Gamma> \<turnstile>\<^sub>s SApp e : \<Gamma>',t \<rightarrow> t'"
-inductive_cases [elim]: "\<Gamma> \<turnstile>\<^sub>s SBind : \<Gamma>',t \<rightarrow> t'"
-inductive_cases [elim]: "\<Gamma> \<turnstile>\<^sub>s SProj l : \<Gamma>',t \<rightarrow> t'"
-inductive_cases [elim]: "\<Gamma> \<turnstile>\<^sub>s SCase tt cs : \<Gamma>',t \<rightarrow> t'"
-inductive_cases [elim]: "\<Gamma> \<turnstile>\<^sub>s SUnfold tt : \<Gamma>',t \<rightarrow> t'"
-inductive_cases [elim]: "\<Gamma> \<turnstile>\<^sub>s STyApp tt : \<Gamma>',t \<rightarrow> t'"
+inductive_cases [elim]: "\<Delta>,\<Gamma> \<turnstile>\<^sub>v VAbs t\<^sub>1 e : t"
+inductive_cases [elim]: "\<Delta>,\<Gamma> \<turnstile>\<^sub>v VRec fs : t"
+inductive_cases [elim]: "\<Delta>,\<Gamma> \<turnstile>\<^sub>v VInj e ts l : t"
+inductive_cases [elim]: "\<Delta>,\<Gamma> \<turnstile>\<^sub>v VFold t' e : t"
+inductive_cases [elim]: "\<Delta>,\<Gamma> \<turnstile>\<^sub>v VTyAbs k e : t"
+inductive_cases [elim]: "\<Delta>,\<Gamma> \<turnstile>\<^sub>v\<^sub>s [] : ts"
+inductive_cases [elim]: "\<Delta>,\<Gamma> \<turnstile>\<^sub>v\<^sub>s v # vs : ts"
+
+inductive typecheck_frame :: "type list \<Rightarrow> frame \<Rightarrow> type \<Rightarrow> type \<Rightarrow> bool" (infix "\<turnstile>\<^sub>s _ : _ \<rightarrow>" 60) where
+  tc_sref [simp]: "lookup x \<Gamma> = Some t \<Longrightarrow> \<Gamma> \<turnstile>\<^sub>s SRef x : t \<rightarrow> t"
+| tc_sapp [simp]: "[],\<Gamma> \<turnstile> e : t' \<Longrightarrow> \<Gamma> \<turnstile>\<^sub>s SApp e : Arrow t' t \<rightarrow> t"
+| tc_sproj [simp]: "lookup l ts = Some t \<Longrightarrow> \<Gamma> \<turnstile>\<^sub>s SProj l : Record ts \<rightarrow> t"
+| tc_scase [simp]: "[],\<Gamma> \<turnstile>\<^sub>c cs : ts \<rightarrow> t \<Longrightarrow> \<Gamma> \<turnstile>\<^sub>s SCase t cs : Variant ts \<rightarrow> t"
+| tc_sunfold [simp]: "[k] \<turnstile>\<^sub>k t : Star \<Longrightarrow> 
+    \<Gamma> \<turnstile>\<^sub>s SUnfold t : Inductive k t \<rightarrow> subst\<^sub>t\<^sub>t 0 (Inductive k t) t"
+| tc_styapp [simp]: "[] \<turnstile>\<^sub>k t' : k \<Longrightarrow> \<Gamma> \<turnstile>\<^sub>s STyApp t' : Forall k t \<rightarrow> subst\<^sub>t\<^sub>t 0 t' t"
+
+inductive_cases [elim]: "\<Gamma> \<turnstile>\<^sub>s SRef x : t \<rightarrow> t'"
+inductive_cases [elim]: "\<Gamma> \<turnstile>\<^sub>s SApp e : t \<rightarrow> t'"
+inductive_cases [elim]: "\<Gamma> \<turnstile>\<^sub>s SProj l : t \<rightarrow> t'"
+inductive_cases [elim]: "\<Gamma> \<turnstile>\<^sub>s SCase tt cs : t \<rightarrow> t'"
+inductive_cases [elim]: "\<Gamma> \<turnstile>\<^sub>s SUnfold tt : t \<rightarrow> t'"
+inductive_cases [elim]: "\<Gamma> \<turnstile>\<^sub>s STyApp tt : t \<rightarrow> t'"
 
 inductive typecheck_stack :: "type list \<Rightarrow> frame list \<Rightarrow> type \<Rightarrow> type \<Rightarrow> bool" 
     (infix "\<turnstile>\<^sub>s\<^sub>s _ : _ \<rightarrow>" 60) where
-  tcs_nil [simp]: "[] \<turnstile>\<^sub>s\<^sub>s [] : t \<rightarrow> t"
-| tcs_cons [simp]: "\<Gamma> \<turnstile>\<^sub>s f : \<Gamma>',t \<rightarrow> t' \<Longrightarrow> \<Gamma> \<turnstile>\<^sub>s\<^sub>s s : t' \<rightarrow> t'' \<Longrightarrow> \<Gamma>' \<turnstile>\<^sub>s\<^sub>s f # s : t \<rightarrow> t''"
+  tcs_nil [simp]: "\<Gamma> \<turnstile>\<^sub>s\<^sub>s [] : t \<rightarrow> t"
+| tcs_cons [simp]: "\<Gamma> \<turnstile>\<^sub>s f : t \<rightarrow> t' \<Longrightarrow> \<Gamma> \<turnstile>\<^sub>s\<^sub>s s : t' \<rightarrow> t'' \<Longrightarrow> \<Gamma> \<turnstile>\<^sub>s\<^sub>s f # s : t \<rightarrow> t''"
 
 inductive_cases [elim]: "\<Gamma> \<turnstile>\<^sub>s\<^sub>s [] : t \<rightarrow> t'"
 inductive_cases [elim]: "\<Gamma> \<turnstile>\<^sub>s\<^sub>s f # s : t \<rightarrow> t'"
 
-inductive typecheck_heap :: "expr list \<Rightarrow> type list \<Rightarrow> bool" 
-    (infix "\<turnstile>\<^sub>h" 60) where
-  tch_nil [simp]: "[] \<turnstile>\<^sub>h []"
-| tch_cons [simp]: "[],\<Gamma> \<turnstile> e : t \<Longrightarrow> h \<turnstile>\<^sub>h \<Gamma> \<Longrightarrow> e # h \<turnstile>\<^sub>h t # \<Gamma>"
+inductive typecheck_heap :: "expr heap \<Rightarrow> type list \<Rightarrow> bool" (infix "\<turnstile>\<^sub>h" 60) where
+  tch_heap [simp]: "(\<And>i t. lookup i \<Gamma> = Some t \<Longrightarrow> [],\<Gamma> \<turnstile> lookup\<^sub>h i h : t) \<Longrightarrow> 
+    length\<^sub>h h = length \<Gamma> \<Longrightarrow> h \<turnstile>\<^sub>h \<Gamma>"
 
-inductive_cases [elim]: "[] \<turnstile>\<^sub>h \<Gamma>"
-inductive_cases [elim]: "e # h \<turnstile>\<^sub>h \<Gamma>"
-inductive_cases [elim]: "h \<turnstile>\<^sub>h []"
-inductive_cases [elim]: "h \<turnstile>\<^sub>h t # \<Gamma>"
+inductive_cases [elim]: "h \<turnstile>\<^sub>h \<Gamma>"
 
 inductive typecheck_stack_state :: "stack_state \<Rightarrow> type \<Rightarrow> bool" (infix "hastype" 60) where
-  tc_stack_state [simp]: "\<Gamma> \<turnstile>\<^sub>s\<^sub>s s : t \<rightarrow> t' \<Longrightarrow> [],\<Gamma> \<turnstile> e : t \<Longrightarrow> h \<turnstile>\<^sub>h \<Gamma> \<Longrightarrow> 
-    (m = Return \<longrightarrow> is_value e) \<Longrightarrow> StackState m e s h hastype t'"
+  tc_eval_state [simp]: "\<Gamma> \<turnstile>\<^sub>s\<^sub>s s : t \<rightarrow> t' \<Longrightarrow> [],\<Gamma> \<turnstile> e : t \<Longrightarrow> h \<turnstile>\<^sub>h \<Gamma> \<Longrightarrow> 
+    StackState (Eval e) s h hastype t'"
+| tc_return_state [simp]: "\<Gamma> \<turnstile>\<^sub>s\<^sub>s s : t \<rightarrow> t' \<Longrightarrow> [],\<Gamma> \<turnstile>\<^sub>v v : t \<Longrightarrow> h \<turnstile>\<^sub>h \<Gamma> \<Longrightarrow> 
+    StackState (Return v) s h hastype t'"
 
-inductive_cases [elim]: "StackState m e s h hastype t"
+inductive_cases [elim]: "StackState (Eval e) s h hastype t"
+inductive_cases [elim]: "StackState (Return v) s h hastype t"
 
-lemma [simp]: "h \<turnstile>\<^sub>h \<Gamma> \<Longrightarrow> lookup x \<Gamma> = Some t \<Longrightarrow> [],\<Gamma> \<turnstile> e : t \<Longrightarrow> update_at x e h \<turnstile>\<^sub>h \<Gamma>"
-  proof (induction h \<Gamma> arbitrary: x rule: typecheck_heap.induct)
-  case (tch_cons \<Gamma> e' t' h)
-    thus ?case
-      proof (induction x)
-      case 0
-        thus ?case by simp
-      next case (Suc x)
-        from Suc have "[] ,\<Gamma> \<turnstile> e' : t'" by simp
-        from Suc have "h \<turnstile>\<^sub>h \<Gamma>" by simp
-        from Suc have "[] ,\<Gamma> \<turnstile> e : t \<Longrightarrow> update_at x e h \<turnstile>\<^sub>h \<Gamma>" by simp
-        from Suc have "lookup x \<Gamma> = Some t" by simp
-        from Suc have "[] ,t' # \<Gamma> \<turnstile> e : t" by simp
+lemma [simp]: "h \<turnstile>\<^sub>h \<Gamma> \<Longrightarrow> lookup x \<Gamma> = Some t \<Longrightarrow> [],\<Gamma> \<turnstile> e : t \<Longrightarrow> update\<^sub>h h x e \<turnstile>\<^sub>h \<Gamma>"
+  proof (induction h \<Gamma> rule: typecheck_heap.induct)
+  case (tch_heap \<Gamma> h)
+    hence "\<And>i t. lookup i \<Gamma> = Some t \<Longrightarrow> [],\<Gamma> \<turnstile> lookup\<^sub>h i (update\<^sub>h h x e) : t" by auto
+    moreover from tch_heap have "length\<^sub>h (update\<^sub>h h x e) = length \<Gamma>" by simp
+    ultimately show ?case by (metis typecheck_heap.tch_heap)
+  qed
 
-
-        have "[],\<Gamma> \<turnstile> e' : t' \<Longrightarrow> update_at x e h \<turnstile>\<^sub>h \<Gamma> \<Longrightarrow> 
-              e' # update_at x e h \<turnstile>\<^sub>h t' # \<Gamma>" by simp
-
-        have "e' # update_at x e h \<turnstile>\<^sub>h t' # \<Gamma>" by simp
-        thus ?case by simp
-      qed
+lemma tc_devalue [simp]: "\<Delta>,\<Gamma> \<turnstile>\<^sub>v v : t \<Longrightarrow> \<Delta>,\<Gamma> \<turnstile> devalue v : t"
+  and "\<Delta>,\<Gamma> \<turnstile>\<^sub>v\<^sub>s vs : ts \<Longrightarrow> \<Delta>,\<Gamma> \<turnstile>\<^sub>f map Var vs : ts"
+  proof (induction \<Delta> \<Gamma> v t and \<Delta> \<Gamma> vs ts rule: typecheck_value_typecheck_vars.inducts)
+  case (tc_vinj x \<Gamma> t l ts \<Delta>)
+    hence "\<Delta>,\<Gamma> \<turnstile> Var x : t" by simp
+    moreover from tc_vinj have "lookup l ts = Some t" by simp
+    moreover from tc_vinj have "\<forall>tt \<in> set ts. \<Delta> \<turnstile>\<^sub>k tt : Star" by simp
+    ultimately show ?case by simp
   qed simp_all
 
-lemma [simp]: "\<Gamma> \<turnstile>\<^sub>s\<^sub>s s : t \<rightarrow> t' \<Longrightarrow> [],\<Gamma> \<turnstile> e : t \<Longrightarrow> h \<turnstile>\<^sub>h \<Gamma> \<Longrightarrow> [],[] \<turnstile> unstack e s h : t'"
+lemma tc_unstack [simp]: "\<Gamma> \<turnstile>\<^sub>s\<^sub>s s : t \<rightarrow> t' \<Longrightarrow> [],\<Gamma> \<turnstile> e : t \<Longrightarrow> h \<turnstile>\<^sub>h \<Gamma> \<Longrightarrow> [],\<Gamma> \<turnstile> unstack e s h : t'"
   proof (induction \<Gamma> s t t' arbitrary: e h rule: typecheck_stack.induct)
-  case (tcs_cons \<Gamma> f \<Gamma>' t t' s t'')
-    thus ?case
-      proof (induction \<Gamma> f \<Gamma>' t t' rule: typecheck_frame.induct)
-      case (tc_sbind \<Gamma> t' t) 
-        moreover then obtain v h' where "h = v # h' \<and> ([],\<Gamma> \<turnstile> v : t') \<and> (h' \<turnstile>\<^sub>h \<Gamma>)" 
-          by fastforce
-        moreover from tc_sbind have "[],insert_at 0 t' \<Gamma> \<turnstile> e : t" by (induction \<Gamma>) simp_all
-        ultimately show ?case by auto
-      qed simp_all
+  case (tcs_cons \<Gamma> f t t' s t'')
+    thus ?case by (induction \<Gamma> f t t' rule: typecheck_frame.induct) simp_all
   qed simp_all
 
-lemma [simp]: "\<Sigma> hastype t \<Longrightarrow> [],[] \<turnstile> unstack_state \<Sigma> : t"
-  by (induction \<Sigma> t rule: typecheck_stack_state.induct) simp_all
+lemma tc_unstack_state [simp]: "\<Sigma> hastype t \<Longrightarrow> \<exists>\<Gamma>. [],\<Gamma> \<turnstile> unstack_state \<Sigma> : t"
+  by (induction \<Sigma> t rule: typecheck_stack_state.induct) 
+     (simp, meson tc_unstack tc_devalue)+
+
+lemma [simp]: "h \<turnstile>\<^sub>h \<Gamma> \<Longrightarrow> [],\<Gamma> \<turnstile> e : t \<Longrightarrow> extend\<^sub>h h e \<turnstile>\<^sub>h insert_at (length\<^sub>h h) t \<Gamma>"
+  proof (induction h \<Gamma> rule: typecheck_heap.induct)
+  case (tch_heap \<Gamma> h)
+    moreover hence "\<And>i tt. lookup i (insert_at (length\<^sub>h h) t \<Gamma>) = Some tt \<Longrightarrow> 
+        [],insert_at (length\<^sub>h h) t \<Gamma> \<turnstile> lookup\<^sub>h i (extend\<^sub>h h e) : tt"
+      using lookup_less_than by fastforce
+    ultimately show ?case by simp
+  qed
+
+lemma [elim]: "h \<turnstile>\<^sub>h \<Gamma> \<Longrightarrow> length\<^sub>h h = length \<Gamma>"
+  by (induction h \<Gamma> rule: typecheck_heap.induct) simp_all
+
+lemma tc_frame_weaken [simp]: "\<Gamma> \<turnstile>\<^sub>s f : t \<rightarrow> t' \<Longrightarrow> insert_at (length \<Gamma>) tt \<Gamma> \<turnstile>\<^sub>s f : t \<rightarrow> t'"
+  by (induction \<Gamma> f t t' rule: typecheck_frame.induct) simp_all
+
+lemma tc_stack_weaken [simp]: "\<Gamma> \<turnstile>\<^sub>s\<^sub>s s : t \<rightarrow> t' \<Longrightarrow> insert_at (length \<Gamma>) tt \<Gamma> \<turnstile>\<^sub>s\<^sub>s s : t \<rightarrow> t'"
+  proof (induction \<Gamma> s t t' rule: typecheck_stack.induct)
+  case (tcs_cons \<Gamma> f t t' s t'')
+    hence "insert_at (length \<Gamma>) tt \<Gamma> \<turnstile>\<^sub>s\<^sub>s s : t' \<rightarrow> t''" by simp
+    moreover from tcs_cons have "insert_at (length \<Gamma>) tt \<Gamma> \<turnstile>\<^sub>s f : t \<rightarrow> t'" by simp
+    ultimately show ?case by simp
+  qed simp_all
 
 end
