02Stack/EvaluateStack.thy
@@ -3,107 +3,177 @@ imports TypecheckStack
 begin
 
 inductive evaluate :: "stack_state \<Rightarrow> stack_state \<Rightarrow> bool" (infix "\<leadsto>\<^sub>s" 60) where
-  ev_abs [simp]: "StackState Eval (Abs t e) s h \<leadsto>\<^sub>s StackState Return (Abs t e) s h"
-| ev_app [simp]: "StackState Eval (App e\<^sub>1 e\<^sub>2) s h \<leadsto>\<^sub>s StackState Eval e\<^sub>1 (SApp e\<^sub>2 # s) h" 
-| ev_let [simp]: "StackState Eval (Let e\<^sub>1 e\<^sub>2) s h \<leadsto>\<^sub>s StackState Eval e\<^sub>2' (SBind # s) (e\<^sub>1 # h)"
-| ev_rec [simp]: "list_all is_var vs \<Longrightarrow> \<not> is_var e \<Longrightarrow> 
-    StackState Eval (Rec (vs @ [e] @ nvs)) s h \<leadsto>\<^sub>s 
-      StackState Eval (Rec (map (incr\<^sub>e\<^sub>e 0) vs @ [Var 0] @ map (incr\<^sub>e\<^sub>e 0) nvs)) (SBind # s) (e # h)" 
-| ev_rec2 [simp]: "list_all is_var vs \<Longrightarrow> \<not> is_var e \<Longrightarrow> 
-    StackState Eval (Rec vs) s h \<leadsto>\<^sub>s StackState Return (Rec vs) s h" 
-| ev_proj [simp]: "StackState Eval (Proj e l) s h \<leadsto>\<^sub>s StackState Eval e (SProj l # s) h"
-| ev_inj [simp]: "StackState Eval (Inj l ts e) s h \<leadsto>\<^sub>s 
-    StackState Return (if is_var e then Inj l ts e else Inj l ts (Var 0)) s h"
-| ev_case [simp]: "StackState Eval (Case e t cs) s h \<leadsto>\<^sub>s StackState Eval e (SCase t cs # s) h"
-| ev_fold [simp]: "StackState Eval (Fold t e) s h \<leadsto>\<^sub>s 
-    StackState Return (if is_var e then Fold t e else Let e (Fold t (Var 0))) s h" 
-| ev_unfold [simp]: "StackState Eval (Unfold t e) s h \<leadsto>\<^sub>s StackState Eval e (SUnfold t # s) h"  
-| ev_tyabs [simp]: "StackState Eval (TyAbs k e) s h \<leadsto>\<^sub>s StackState Return (TyAbs k e) s h" 
-| ev_tyapp [simp]: "StackState Eval (TyApp e t) s h \<leadsto>\<^sub>s StackState Eval e (STyApp t # s) h" 
-| ev_tylet [simp]: "StackState Eval (TyLet t e) s h \<leadsto>\<^sub>s StackState Eval (subst\<^sub>t\<^sub>e 0 t e) s h" 
+  ev_var [simp]: "StackState (Eval (Var x)) s h \<leadsto>\<^sub>s StackState (Eval (lookup\<^sub>h x h)) (SRef x # s) h"
+| ev_abs [simp]: "StackState (Eval (Abs t e)) s h \<leadsto>\<^sub>s StackState (Return (VAbs t e)) s h"
+| ev_app [simp]: "StackState (Eval (App e\<^sub>1 e\<^sub>2)) s h \<leadsto>\<^sub>s StackState (Eval e\<^sub>1) (SApp e\<^sub>2 # s) h" 
+| ev_let [simp]: "StackState (Eval (Let e\<^sub>1 e\<^sub>2)) s h \<leadsto>\<^sub>s 
+    StackState (Eval (subst\<^sub>e\<^sub>e 0 (Var (length\<^sub>h h)) e\<^sub>2)) s (extend\<^sub>h h e\<^sub>1)"
+| ev_rec1 [simp]: "list_all is_var vs \<Longrightarrow> \<not> is_var e \<Longrightarrow> 
+    StackState (Eval (Rec (vs @ [e] @ nvs))) s h \<leadsto>\<^sub>s 
+      StackState (Eval (Rec (vs @ [Var (length\<^sub>h h)] @ nvs))) s (extend\<^sub>h h e)" 
+| ev_rec2 [simp]: "list_all is_var vs \<Longrightarrow>
+    StackState (Eval (Rec vs)) s h \<leadsto>\<^sub>s StackState (Return (VRec (map devar vs))) s h" 
+| ev_proj [simp]: "StackState (Eval (Proj e l)) s h \<leadsto>\<^sub>s StackState (Eval e) (SProj l # s) h"
+| ev_inj1 [simp]: "StackState (Eval (Inj l ts (Var x))) s h \<leadsto>\<^sub>s StackState (Return (VInj l ts x)) s h"
+| ev_inj2 [simp]: "\<not> is_var e \<Longrightarrow> StackState (Eval (Inj l ts e)) s h \<leadsto>\<^sub>s 
+    StackState (Return (VInj l ts (length\<^sub>h h))) s (extend\<^sub>h h e)"
+| ev_case [simp]: "StackState (Eval (Case e t cs)) s h \<leadsto>\<^sub>s StackState (Eval e) (SCase t cs # s) h"
+| ev_fold1 [simp]: "StackState (Eval (Fold t (Var x))) s h \<leadsto>\<^sub>s StackState (Return (VFold t x)) s h" 
+| ev_fold2 [simp]: "\<not> is_var e \<Longrightarrow> 
+    StackState (Eval (Fold t e)) s h \<leadsto>\<^sub>s StackState (Return (VFold t (length\<^sub>h h))) s (extend\<^sub>h h e)" 
+| ev_unfold [simp]: "StackState (Eval (Unfold t e)) s h \<leadsto>\<^sub>s StackState (Eval e) (SUnfold t # s) h"  
+| ev_tyabs [simp]: "StackState (Eval (TyAbs k e)) s h \<leadsto>\<^sub>s StackState (Return (VTyAbs k e)) s h" 
+| ev_tyapp [simp]: "StackState (Eval (TyApp e t)) s h \<leadsto>\<^sub>s StackState (Eval e) (STyApp t # s) h" 
+| ev_tylet [simp]: "StackState (Eval (TyLet t e)) s h \<leadsto>\<^sub>s StackState (Eval (subst\<^sub>t\<^sub>e 0 t e)) s h" 
+| ret_ref [simp]: "StackState (Return v) (SRef x # s) h \<leadsto>\<^sub>s StackState (Return v) s (update\<^sub>h h x e)"
 | ret_app [simp]: 
-    "StackState Return (Abs t e\<^sub>1) (SApp e\<^sub>2 # s) h \<leadsto>\<^sub>s StackState Eval e\<^sub>1 (SBind # s) (e\<^sub>2 # h)"
-| ret_proj [simp]: "lookup l fs = Some e \<Longrightarrow> 
-    StackState Return (Rec fs) (SProj l # s) h \<leadsto>\<^sub>s StackState Eval e s h" 
-| ret_case [simp]: "lookup l cs = Some e' \<Longrightarrow> 
-    StackState Return (Inj l ts e) (SCase t cs # s) h \<leadsto>\<^sub>s StackState Eval e' (SBind # s) (e # h)"
-| ret_unfold [simp]: "StackState Return (Fold t e) (SUnfold t # s) h \<leadsto>\<^sub>s StackState Eval e s h" 
+    "StackState (Return (VAbs t e\<^sub>1)) (SApp e\<^sub>2 # s) h \<leadsto>\<^sub>s StackState (Eval e\<^sub>1) s (extend\<^sub>h h e\<^sub>2)"
+| ret_proj [simp]: "lookup l xs = Some x \<Longrightarrow> 
+    StackState (Return (VRec xs)) (SProj l # s) h \<leadsto>\<^sub>s StackState (Eval (Var x)) s h" 
+| ret_case [simp]: "lookup l cs = Some e \<Longrightarrow> 
+    StackState (Return (VInj l ts x)) (SCase t cs # s) h \<leadsto>\<^sub>s 
+      StackState (Eval e) s (extend\<^sub>h h (Var x))"
+| ret_unfold [simp]: 
+    "StackState (Return (VFold t e)) (SUnfold t # s) h \<leadsto>\<^sub>s StackState (Eval (Var e)) s h" 
 | ret_tyapp [simp]: 
-    "StackState Return (TyAbs k e) (STyApp t # s) h \<leadsto>\<^sub>s StackState Eval (subst\<^sub>t\<^sub>e 0 t e) s h" 
-| ret_app_let [simp]: "StackState Return (Let e\<^sub>1\<^sub>1 e\<^sub>1\<^sub>2) (SApp e\<^sub>2 # s) h \<leadsto>\<^sub>s 
-    StackState Eval e\<^sub>1\<^sub>2 (SApp (incr\<^sub>e\<^sub>e 0 e\<^sub>2) # SBind # s) (e\<^sub>1\<^sub>1 # h)"
-| ret_proj_let [simp]: "StackState Return (Let e\<^sub>1 e\<^sub>2) (SProj l # s) h \<leadsto>\<^sub>s 
-    StackState Eval e\<^sub>2 (SProj l # SBind # s) (e\<^sub>1 # h)" 
-| ret_case_let [simp]: "StackState Return (Let e\<^sub>1 e\<^sub>2) (SCase t cs # s) h \<leadsto>\<^sub>s 
-    StackState Eval e\<^sub>2 (SCase t (map (incr\<^sub>e\<^sub>e (Suc 0)) cs) # SBind # s) (e\<^sub>1 # h)" 
-| ret_unfold_let [simp]: "StackState Return (Let e\<^sub>1 e\<^sub>2) (SUnfold t # s) h \<leadsto>\<^sub>s 
-    StackState Eval e\<^sub>2 (SUnfold t # SBind # s) (e\<^sub>1 # h)"
-| ret_tyapp_let [simp]: "StackState Return (Let e\<^sub>1 e\<^sub>2) (STyApp t # s) h \<leadsto>\<^sub>s 
-    StackState Eval e\<^sub>2 (STyApp t # SBind # s) (e\<^sub>1 # h)" 
+    "StackState (Return (VTyAbs k e)) (STyApp t # s) h \<leadsto>\<^sub>s StackState (Eval (subst\<^sub>t\<^sub>e 0 t e)) s h" 
 
-primrec is_final :: "stack_state \<Rightarrow> bool" where
-  "is_final (StackState m e s h) = (m = Return \<and> s = [])"
+fun is_final :: "stack_state \<Rightarrow> bool" where
+  "is_final (StackState (Return v) [] h) = True"
+| "is_final (StackState (Return v) (f # s) h) = False"
+| "is_final (StackState (Eval e) s h) = False"
+
+lemma vcanonical_arrow [simp]: "\<Delta>,\<Gamma> \<turnstile>\<^sub>v v : Arrow t\<^sub>1 t\<^sub>2 \<Longrightarrow> \<exists>e. v = VAbs t\<^sub>1 e"
+  by (induction \<Gamma> v "Arrow t\<^sub>1 t\<^sub>2" rule: typecheck_value_typecheck_vars.inducts(1)) simp_all
+
+lemma vcanonical_record [simp]: "\<Delta>,\<Gamma> \<turnstile>\<^sub>v v : Record ts \<Longrightarrow> \<exists>vs. v = VRec vs \<and> \<Delta>,\<Gamma> \<turnstile>\<^sub>v\<^sub>s vs : ts"
+  by (induction \<Gamma> v "Record ts" rule: typecheck_value_typecheck_vars.inducts(1)) simp_all
+
+lemma vcanonical_variant [simp]: "\<Delta>,\<Gamma> \<turnstile>\<^sub>v v : Variant ts \<Longrightarrow> \<exists>l x. v = VInj l ts x \<and> l < length ts"
+  by (induction \<Gamma> v "Variant ts" rule: typecheck_value_typecheck_vars.inducts(1)) auto
+
+lemma vcanonical_inductive [simp]: "\<Delta>,\<Gamma> \<turnstile>\<^sub>v v : Inductive k t \<Longrightarrow> \<exists>x. v = VFold t x"
+  by (induction \<Gamma> v "Inductive k t" rule: typecheck_value_typecheck_vars.inducts(1)) auto
+
+lemma vcanonical_forall [simp]: "\<Delta>,\<Gamma> \<turnstile>\<^sub>v v : Forall k t \<Longrightarrow> \<exists>e. v = VTyAbs k e"
+  by (induction \<Gamma> v "Forall k t" rule: typecheck_value_typecheck_vars.inducts(1)) auto
+
+lemma lookup_in_tc [simp]: "\<Delta>,\<Gamma> \<turnstile>\<^sub>v\<^sub>s xs : ts \<Longrightarrow> lookup l ts = Some t \<Longrightarrow> \<exists>x. lookup l xs = Some x"
+  by (induction l xs arbitrary: ts rule: lookup.induct) auto
+
+lemma "\<Delta>,\<Gamma> \<turnstile> e : t \<Longrightarrow> True"
+  and "\<Delta>,\<Gamma> \<turnstile>\<^sub>f fs : ts \<Longrightarrow> True"
+  and lookup_in_cs [simp]: "\<Delta>,\<Gamma> \<turnstile>\<^sub>c cs : ts \<rightarrow> t \<Longrightarrow> l < length ts \<Longrightarrow> \<exists>e. lookup l cs = Some e"
+  proof (induction \<Delta> \<Gamma> e t and \<Delta> \<Gamma> fs ts and \<Delta> \<Gamma> cs ts t arbitrary: and and l 
+         rule: typecheck_typecheck_fs_typecheck_cs.inducts)
+  case tcc_cons
+    thus ?case by (induction l) simp_all
+  qed simp_all
 
 theorem progress: "\<Sigma> hastype t \<Longrightarrow> is_final \<Sigma> \<or> (\<exists>\<Sigma>'. \<Sigma> \<leadsto>\<^sub>s \<Sigma>')"
   proof (induction \<Sigma> t rule: typecheck_stack_state.induct)
-  case (tc_stack_state \<Gamma> s t t' e h m)
+  case (tc_eval_state \<Gamma> s t t' e h)
     thus ?case
-      proof (induction m)
-      case Eval
-        thus ?case
-          proof (induction e)
-          case Var
-            thus ?case by simp
-          next case Abs
-            thus ?case by (metis ev_abs)
-          next case App
-            thus ?case by (metis ev_app)
-          next case Let
-            thus ?case by (metis ev_let)
-          next case Rec
-            thus ?case by (metis ev_app)
-          next case Proj
-            thus ?case by (metis ev_proj)
-          next case Inj 
-            thus ?case by (metis ev_inj)
-          next case Case
-            thus ?case by (metis ev_case)
-          next case Fold 
-            thus ?case by (metis ev_fold)
-          next case Unfold
-            thus ?case by (metis ev_unfold)
-          next case TyAbs
-            thus ?case by (metis ev_tyabs)
-          next case TyApp
-            thus ?case by (metis ev_tyapp)
-          next case TyLet
-            thus ?case by (metis ev_tylet)
-          qed
-      next case Return
-        thus ?case
-          proof (induction \<Gamma> s t t' rule: typecheck_stack.induct)
-          case (tcs_cons \<Gamma> f \<Gamma>' t t' s t'')
-            from tcs_cons have "\<Gamma> \<turnstile>\<^sub>s f : \<Gamma>',t \<rightarrow> t'" by simp
-            from tcs_cons have "\<Gamma> \<turnstile>\<^sub>s\<^sub>s s : t' \<rightarrow> t''" by simp
-            from tcs_cons have "[] ,\<Gamma> \<turnstile> e : t' \<Longrightarrow> h \<turnstile>\<^sub>h \<Gamma> \<Longrightarrow> s = [] \<or> (\<exists>a. StackState Return e s h \<leadsto>\<^sub>s a)" by simp
-            from tcs_cons have "[] ,\<Gamma>' \<turnstile> e : t" by simp
-            from tcs_cons have "h \<turnstile>\<^sub>h \<Gamma>'" by simp
-            from tcs_cons have "is_value e" by simp
-        
-        
-            have "StackState Return e (f # s) h \<leadsto>\<^sub>s \<Sigma>'" by simp
-            thus ?case by fastforce
-          qed simp_all
+      proof (induction e)
+      case Var
+        thus ?case by (metis ev_var)
+      next case Abs
+        thus ?case by (metis ev_abs)
+      next case App
+        thus ?case by (metis ev_app)
+      next case Let
+        thus ?case by (metis ev_let)
+      next case Rec
+        thus ?case by (metis split_fields ev_rec1 ev_rec2)
+      next case Proj
+        thus ?case by (metis ev_proj)
+      next case (Inj l ts e) 
+        thus ?case by (cases e) (meson ev_inj1 ev_inj2 is_var.simps)+
+      next case Case
+        thus ?case by (metis ev_case)
+      next case (Fold tt e)
+        thus ?case by (cases e) (meson ev_fold1 ev_fold2 is_var.simps)+
+      next case Unfold
+        thus ?case by (metis ev_unfold)
+      next case TyAbs
+        thus ?case by (metis ev_tyabs)
+      next case TyApp
+        thus ?case by (metis ev_tyapp)
+      next case TyLet
+        thus ?case by (metis ev_tylet)
       qed
+  next case (tc_return_state \<Gamma> s t t' v h)
+    thus ?case
+      proof (induction \<Gamma> s t t' rule: typecheck_stack.induct)
+      case (tcs_cons \<Gamma> f \<Gamma>' t t' s t'')
+        thus ?case
+          proof (induction \<Gamma> f \<Gamma>' t t' rule: typecheck_frame.induct)
+          case tc_sref
+            thus ?case by (metis ret_ref)
+          next case tc_sapp
+            thus ?case by (metis vcanonical_arrow ret_app)
+          next case tc_sproj
+            thus ?case by (metis vcanonical_record ret_proj lookup_in_tc)
+          next case tc_scase
+            thus ?case by (metis vcanonical_variant ret_case lookup_in_cs)
+          next case tc_sunfold
+            thus ?case by (metis vcanonical_inductive ret_unfold)
+          next case tc_styapp
+            thus ?case by (metis vcanonical_forall ret_tyapp)
+          qed
+      qed simp_all
   qed
+
+lemma [simp]: "h \<turnstile>\<^sub>h \<Gamma> \<Longrightarrow> lookup x \<Gamma> = Some t \<Longrightarrow> [],\<Gamma> \<turnstile> lookup\<^sub>h x h : t"
+  by (induction h \<Gamma> rule: typecheck_heap.induct) simp_all
 
 theorem preservation: "\<Sigma> \<leadsto>\<^sub>s \<Sigma>' \<Longrightarrow> \<Sigma> hastype t \<Longrightarrow> \<Sigma>' hastype t"
   proof (induction \<Sigma> \<Sigma>' rule: evaluate.induct)
-  case (ev_app e\<^sub>1 e\<^sub>2 s h)
+  case (ev_var x s h)
+    then obtain \<Gamma> tt where "(\<Gamma> \<turnstile>\<^sub>s\<^sub>s s : tt \<rightarrow> t) \<and> (lookup x \<Gamma> = Some tt) \<and> (h \<turnstile>\<^sub>h \<Gamma>)" by blast
+    moreover hence "\<Gamma> \<turnstile>\<^sub>s\<^sub>s SRef x # s : tt \<rightarrow> t" by (metis tc_sref tcs_cons)
+    ultimately show ?case by simp
+  next case (ev_app e\<^sub>1 e\<^sub>2 s h)
     then obtain \<Gamma> t\<^sub>1 t\<^sub>2 where "(\<Gamma> \<turnstile>\<^sub>s\<^sub>s s : t\<^sub>2 \<rightarrow> t) \<and> ([],\<Gamma> \<turnstile> e\<^sub>1 : Arrow t\<^sub>1 t\<^sub>2) \<and> 
-      ([],\<Gamma> \<turnstile> e\<^sub>2 : t\<^sub>1) \<and> (h \<turnstile>\<^sub>h \<Gamma>)" by fastforce
+      ([],\<Gamma> \<turnstile> e\<^sub>2 : t\<^sub>1) \<and> (h \<turnstile>\<^sub>h \<Gamma>)" by blast
     moreover hence "\<Gamma> \<turnstile>\<^sub>s\<^sub>s SApp e\<^sub>2 # s : Arrow t\<^sub>1 t\<^sub>2 \<rightarrow> t" by (metis tc_sapp tcs_cons)
     ultimately show ?case by simp
-  qed simp_all
+  next case (ev_let e\<^sub>1 e\<^sub>2 s h)
+    then obtain \<Gamma> t\<^sub>1 t\<^sub>2 where T: "(\<Gamma> \<turnstile>\<^sub>s\<^sub>s s : t\<^sub>2 \<rightarrow> t) \<and> ([],\<Gamma> \<turnstile> e\<^sub>1 : t\<^sub>1) \<and> 
+      ([],insert_at 0 t\<^sub>1 \<Gamma> \<turnstile> e\<^sub>2 : t\<^sub>2) \<and> (h \<turnstile>\<^sub>h \<Gamma>)" by blast
+    hence L: "length\<^sub>h h = length \<Gamma>" by blast
+    from T have X: "insert_at (length \<Gamma>) t\<^sub>1 \<Gamma> \<turnstile>\<^sub>s\<^sub>s s : t\<^sub>2 \<rightarrow> t" by simp
+    from T have "[],insert_at (length (insert_at 0 t\<^sub>1 \<Gamma>)) t\<^sub>1 (insert_at 0 t\<^sub>1 \<Gamma>) \<turnstile> e\<^sub>2 : t\<^sub>2" 
+      using tc_weaken by blast
+    with L have Y: "[],insert_at 0 t\<^sub>1 (insert_at (length\<^sub>h h) t\<^sub>1 \<Gamma>) \<turnstile> e\<^sub>2 : t\<^sub>2" by simp
+    from L have "lookup (length\<^sub>h h) (insert_at (length\<^sub>h h) t\<^sub>1 \<Gamma>) = Some t\<^sub>1" by simp
+    with T X Y show ?case by simp
+  next case ev_rec1 
+    thus ?case by metis
+  next case ev_rec2  
+    thus ?case by metis
+  next case ev_proj 
+    thus ?case by metis
+  next case ev_inj2 
+    thus ?case by metis
+  next case ev_case 
+    thus ?case by metis
+  next case ev_fold2 
+    thus ?case by metis
+  next case ev_unfold 
+    thus ?case by metis
+  next case ev_tyapp 
+    thus ?case by metis
+  next case ret_ref 
+    thus ?case by metis
+  next case ret_app 
+    thus ?case by metis
+  next case ret_proj 
+    thus ?case by metis
+  next case ret_case 
+    thus ?case by metis
+  next case ret_tyapp 
+    thus ?case by metis
+  qed fastforce+
 
 end
