Heap.thy
@@ -1,0 +1,31 @@
+theory Heap
+imports Main
+begin
+
+datatype 'a heap = Heap "nat \<Rightarrow> 'a" nat
+
+primrec length\<^sub>h :: "'a heap \<Rightarrow> nat" where
+  "length\<^sub>h (Heap h n) = n"
+
+primrec lookup\<^sub>h :: "nat \<Rightarrow> 'a heap \<Rightarrow>'a" where
+  "lookup\<^sub>h x (Heap h n) = h x"
+
+primrec extend\<^sub>h :: "'a heap \<Rightarrow> 'a \<Rightarrow> 'a heap" where
+  "extend\<^sub>h (Heap h n) a = Heap (h(n := a)) (Suc n)"
+
+primrec update\<^sub>h :: "'a heap \<Rightarrow> nat \<Rightarrow> 'a \<Rightarrow> 'a heap" where
+  "update\<^sub>h (Heap h n) x a = Heap (h(x := a)) n"
+
+lemma [simp]: "length\<^sub>h (extend\<^sub>h h a) = Suc (length\<^sub>h h)"
+  by (induction h) simp_all
+
+lemma [simp]: "length\<^sub>h (update\<^sub>h h x a) = length\<^sub>h h"
+  by (induction h) simp_all 
+
+lemma [simp]: "lookup\<^sub>h y (update\<^sub>h h x a) = (if x = y then a else lookup\<^sub>h y h)"
+  by (induction h) simp_all
+
+lemma [simp]: "lookup\<^sub>h x (extend\<^sub>h h a) = (if x = length\<^sub>h h then a else lookup\<^sub>h x h)"
+  by (induction h) simp_all
+
+end
